better names

WPDS/WAutomaton.thy
@@ -709,23 +709,24 @@ proof (rule HOL.ext)
     using finfun_apply_pair_weight_transition by (cases t) fastforce
 qed
 
-definition intersff :: "('state, 'label::finite, 'weight::bounded_dioid) w_transitions \<Rightarrow> ('state, 'label, 'weight) w_transitions \<Rightarrow> (('state \<times> 'state), 'label, 'weight) w_transitions" where
-  "intersff = (\<lambda>ts1 ts2. (case_prod (*)) \<circ>$ (pair_weight ts1 ts2))"
+(* Weighted Intersection *)
+definition w_inters :: "('state, 'label::finite, 'weight::bounded_dioid) w_transitions \<Rightarrow> ('state, 'label, 'weight) w_transitions \<Rightarrow> (('state \<times> 'state), 'label, 'weight) w_transitions" where
+  "w_inters = (\<lambda>ts1 ts2. (case_prod (*)) \<circ>$ (pair_weight ts1 ts2))"
 
-lemma finfun_apply_intersff_transition:
+lemma finfun_apply_w_inters_transition:
   fixes p1::"'state::finite"
   fixes q1::"'state::finite"
-  shows "intersff ts1 ts2 $ ((p1,q1),\<gamma>,(p2,q2)) = (ts1 $ (p1,\<gamma>,p2)*ts2 $ (q1,\<gamma>,q2))"
-  by (auto simp add: fst_weight_apply snd_weight_apply finfun_apply_pair_weight_transition intersff_def)
+  shows "w_inters ts1 ts2 $ ((p1,q1),\<gamma>,(p2,q2)) = (ts1 $ (p1,\<gamma>,p2)*ts2 $ (q1,\<gamma>,q2))"
+  by (auto simp add: fst_weight_apply snd_weight_apply finfun_apply_pair_weight_transition w_inters_def)
 
-lemma finfun_apply_intersff:
+lemma finfun_apply_w_inters:
   fixes ts1::"('state::finite, 'label::finite, 'weight::bounded_dioid) w_transitions"
   fixes ts2::"('state::finite, 'label, 'weight) w_transitions"
-  shows "(($) (intersff ts1 ts2)) = (\<lambda>t. (ts1 $ (fst_trans t) * ts2 $ (snd_trans t)))"
+  shows "(($) (w_inters ts1 ts2)) = (\<lambda>t. (ts1 $ (fst_trans t) * ts2 $ (snd_trans t)))"
 proof (rule HOL.ext)
   fix t
-  show "intersff ts1 ts2 $ t = ts1 $ (fst_trans t) * ts2 $ (snd_trans t)"
-    using finfun_apply_intersff_transition by (cases t) force
+  show "w_inters ts1 ts2 $ t = ts1 $ (fst_trans t) * ts2 $ (snd_trans t)"
+    using finfun_apply_w_inters_transition by (cases t) force
 qed
 
 lemma inftersff_complete_transition_finfun_apply:
@@ -733,22 +734,22 @@ lemma inftersff_complete_transition_finfun_apply:
   fixes p'::"'state::finite"
   assumes "A $ (p, y, q) = d"
   assumes "A' $ (p', y, q') = d'"
-  shows "(intersff A A') $ ((p,p'), y, (q,q')) = d * d'"
-  using assms finfun_apply_intersff_transition by auto
+  shows "(w_inters A A') $ ((p,p'), y, (q,q')) = d * d'"
+  using assms finfun_apply_w_inters_transition by auto
 
 lemma inftersff_complete_transition:
   fixes p1::"'state::finite"
   fixes q1::"'state::finite"
   assumes "(p1, ([\<alpha>], dp), p') \<in> wts_to_monoidLTS ts1"
   assumes "(q1, ([\<alpha>], dq), q') \<in> wts_to_monoidLTS ts2"
-  shows "((p1, q1), ([\<alpha>], dp * dq), (p', q')) \<in> wts_to_monoidLTS (intersff ts1 ts2)"
-  using assms finfun_apply_intersff_transition[of ts1 ts2 p1 q1 \<alpha> p' q']
+  shows "((p1, q1), ([\<alpha>], dp * dq), (p', q')) \<in> wts_to_monoidLTS (w_inters ts1 ts2)"
+  using assms finfun_apply_w_inters_transition[of ts1 ts2 p1 q1 \<alpha> p' q']
   unfolding wts_to_monoidLTS_def by auto
 
-lemma intersff_sound_transition:
+lemma w_inters_sound_transition:
   fixes ts1::"('state::finite, 'label::finite, 'weight::bounded_dioid) w_transitions"
   fixes ts2::"('state::finite, 'label, 'weight) w_transitions"
-  assumes "((p2, q2), (w23, d23), p3, q3) \<in> wts_to_monoidLTS (intersff ts1 ts2)"
+  assumes "((p2, q2), (w23, d23), p3, q3) \<in> wts_to_monoidLTS (w_inters ts1 ts2)"
   obtains d23p d23q where
     "(p2, (w23, d23p), p3) \<in> wts_to_monoidLTS ts1"
     "(q2, (w23, d23q), q3) \<in> wts_to_monoidLTS ts2"
@@ -757,7 +758,7 @@ proof -
   have "\<exists>d23p d23q. ts1 $ (p2, (hd w23), p3) = d23p \<and>
                     ts2 $ (q2, (hd w23), q3) = d23q \<and>
                     d23 = d23p * d23q"
-    using assms finfun_apply_intersff_transition wts_label_d' by fastforce
+    using assms finfun_apply_w_inters_transition wts_label_d' by fastforce
   then show ?thesis
     by (metis wts_to_monoidLTS_exists_iff assms list.sel(1) that wts_label_d)
 qed
@@ -818,12 +819,12 @@ next
     using binary_aut_transition_binary by fastforce
 qed
 
-lemma intersff_complete_exi:
+lemma w_inters_complete_exi:
   fixes ts1::"('state::finite, 'label::finite, 'weight::bounded_dioid) w_transitions"
   fixes ts2::"('state::finite, 'label, 'weight) w_transitions"
   assumes "(p1, (w,dp), p2) \<in> monoid_rtrancl (wts_to_monoidLTS ts1)"
   assumes "(q1, (w,dq), q2) \<in> monoid_rtrancl (wts_to_monoidLTS ts2)"
-  shows "\<exists>d. ((p1,q1), (w,d), (p2,q2)) \<in> monoid_rtrancl (wts_to_monoidLTS (intersff ts1 ts2))"
+  shows "\<exists>d. ((p1,q1), (w,d), (p2,q2)) \<in> monoid_rtrancl (wts_to_monoidLTS (w_inters ts1 ts2))"
   using assms 
 proof (induction w arbitrary: p1 q1 dp dq)
   case Nil
@@ -837,27 +838,27 @@ next
     by (meson Cons.prems(1) Cons.prems(2) monoid_rtrancl_wts_to_monoidLTS_cases_rev)
   then have "ts1 $ (p1, \<gamma>, p') = dp1" "ts2 $ (q1, \<gamma>, q') = dq1"
     by (simp add: wts_label_d)+
-  then have "(intersff ts1 ts2) $ ((p1,q1), \<gamma>, (p',q')) = dp1 * dq1"
-    using finfun_apply_intersff_transition by blast
-  then have pq1_pq1: "((p1,q1), ([\<gamma>], dp1 * dq1), (p',q')) \<in> wts_to_monoidLTS (intersff ts1 ts2)"
+  then have "(w_inters ts1 ts2) $ ((p1,q1), \<gamma>, (p',q')) = dp1 * dq1"
+    using finfun_apply_w_inters_transition by blast
+  then have pq1_pq1: "((p1,q1), ([\<gamma>], dp1 * dq1), (p',q')) \<in> wts_to_monoidLTS (w_inters ts1 ts2)"
     by (simp add: wts_to_monoidLTS_def)
   from pq'_p Cons(1) obtain d2 where d2_p:
-    "((p',q'), (w, d2), (p2,q2)) \<in> monoid_rtrancl (wts_to_monoidLTS (intersff ts1 ts2))"
+    "((p',q'), (w, d2), (p2,q2)) \<in> monoid_rtrancl (wts_to_monoidLTS (w_inters ts1 ts2))"
     by blast
-  then have "((p1,q1), (\<gamma>#w, (dp1 * dq1)*d2), (p2,q2)) \<in> monoid_rtrancl (wts_to_monoidLTS (intersff ts1 ts2))"
-    using monoid_rtrancl_into_rtrancl_rev[of "(p1,q1)" "([\<gamma>],dp1 * dq1)" "(p',q')" "wts_to_monoidLTS (intersff ts1 ts2)" "(w,d2)" "(p2,q2)"]
+  then have "((p1,q1), (\<gamma>#w, (dp1 * dq1)*d2), (p2,q2)) \<in> monoid_rtrancl (wts_to_monoidLTS (w_inters ts1 ts2))"
+    using monoid_rtrancl_into_rtrancl_rev[of "(p1,q1)" "([\<gamma>],dp1 * dq1)" "(p',q')" "wts_to_monoidLTS (w_inters ts1 ts2)" "(w,d2)" "(p2,q2)"]
     using pq1_pq1 by auto
   then show ?case
     by auto
 qed
 
-lemma intersff_complete_1:
+lemma w_inters_complete_1:
   fixes p1::"'state::finite"
   fixes q1::"'state::finite"
   assumes "(p1, (w,1), p2) \<in> monoid_rtrancl (wts_to_monoidLTS ts1)"
   assumes "(q1, (w,d), q2) \<in> monoid_rtrancl (wts_to_monoidLTS ts2)"
   assumes "binary_aut ts1"
-  shows "((p1,q1), (w,d), (p2,q2)) \<in> monoid_rtrancl (wts_to_monoidLTS (intersff ts1 ts2))"
+  shows "((p1,q1), (w,d), (p2,q2)) \<in> monoid_rtrancl (wts_to_monoidLTS (w_inters ts1 ts2))"
   using assms(1,2)
 proof (induction w arbitrary: p1 q1 d)
   case (Cons \<alpha> w1')
@@ -870,14 +871,14 @@ proof (induction w arbitrary: p1 q1 d)
     "(q', (w1',dq'q2), q2) \<in> monoid_rtrancl (wts_to_monoidLTS ts2)"
     "d = dq1q' * dq'q2"
     using Cons(3) using monoid_rtrancl_wts_to_monoidLTS_cases_rev[of q1 \<alpha> w1' d q2 ts2] by meson
-  have ind: "((p', q'), (w1', dq'q2), (p2, q2)) \<in> monoid_rtrancl (wts_to_monoidLTS (intersff ts1 ts2))"
+  have ind: "((p', q'), (w1', dq'q2), (p2, q2)) \<in> monoid_rtrancl (wts_to_monoidLTS (w_inters ts1 ts2))"
     by (simp add: Cons.IH p'_p(2) q'_p(2))
   moreover
-  have "((p1, q1), ([\<alpha>], dq1q'), (p', q')) \<in> (wts_to_monoidLTS (intersff ts1 ts2))"
+  have "((p1, q1), ([\<alpha>], dq1q'), (p', q')) \<in> (wts_to_monoidLTS (w_inters ts1 ts2))"
     using p'_p q'_p inftersff_complete_transition by (metis mult_1)
   ultimately
-  have "((p1, q1), (\<alpha>#w1', dq1q' * dq'q2), (p2, q2)) \<in> monoid_rtrancl (wts_to_monoidLTS (intersff ts1 ts2))"
-    using monoid_rtrancl_into_rtrancl_rev[of "(p1, q1)" " ([\<alpha>], dq1q')" "(p', q')" "wts_to_monoidLTS (intersff ts1 ts2)" "(w1', dq'q2)" "(p2, q2)"]
+  have "((p1, q1), (\<alpha>#w1', dq1q' * dq'q2), (p2, q2)) \<in> monoid_rtrancl (wts_to_monoidLTS (w_inters ts1 ts2))"
+    using monoid_rtrancl_into_rtrancl_rev[of "(p1, q1)" " ([\<alpha>], dq1q')" "(p', q')" "wts_to_monoidLTS (w_inters ts1 ts2)" "(w1', dq'q2)" "(p2, q2)"]
     by simp
   then show ?case
     by (simp add: q'_p)
@@ -887,13 +888,13 @@ next
     by (metis fst_conv monoid_rtrancl.monoid_rtrancl_refl monoid_star_w0 mstar_wts_empty_one one_list_def one_prod_def)
 qed
 
-lemma intersff_complete_0:
+lemma w_inters_complete_0:
   fixes ts1::"('state::finite, 'label::finite, 'weight::bounded_dioid) w_transitions"
   fixes ts2::"('state::finite, 'label, 'weight) w_transitions"
   assumes "(p1, (w,0), p2) \<in> monoid_rtrancl (wts_to_monoidLTS ts1)"
   assumes "(q1, (w,d), q2) \<in> monoid_rtrancl (wts_to_monoidLTS ts2)"
   assumes "binary_aut ts1"
-  shows "((p1,q1), (w,0), (p2,q2)) \<in> monoid_rtrancl (wts_to_monoidLTS (intersff ts1 ts2))"
+  shows "((p1,q1), (w,0), (p2,q2)) \<in> monoid_rtrancl (wts_to_monoidLTS (w_inters ts1 ts2))"
   using assms(1,2)
 proof (induction w arbitrary: p1 q1 d)
   case (Cons \<alpha> w1')
@@ -913,14 +914,14 @@ proof (induction w arbitrary: p1 q1 d)
       "(q', (w1', qd2), q2) \<in> monoid_rtrancl (wts_to_monoidLTS ts2)"
       using Cons(3) monoid_rtrancl_wts_to_monoidLTS_cases_rev by fastforce
     ultimately
-    have pq1_pq': "((p1,q1), ([\<alpha>], 0), (p',q')) \<in> wts_to_monoidLTS (intersff ts1 ts2)"
+    have pq1_pq': "((p1,q1), ([\<alpha>], 0), (p',q')) \<in> wts_to_monoidLTS (w_inters ts1 ts2)"
       using inftersff_complete_transition by fastforce
 
-    obtain d2 where pq'_pq2: "((p',q'), (w1', d2), (p2,q2)) \<in> monoid_rtrancl (wts_to_monoidLTS (intersff ts1 ts2))"
-      using intersff_complete_exi[of p' w1' _ p2 ts1 q' _ q2 ts2] Cons p'_p(2)
+    obtain d2 where pq'_pq2: "((p',q'), (w1', d2), (p2,q2)) \<in> monoid_rtrancl (wts_to_monoidLTS (w_inters ts1 ts2))"
+      using w_inters_complete_exi[of p' w1' _ p2 ts1 q' _ q2 ts2] Cons p'_p(2)
         q'_p(2) monoid_star_intros_step by blast
     show ?thesis
-      using pq1_pq' pq'_pq2 monoid_rtrancl_into_rtrancl_rev[of "(p1, q1)" "([\<alpha>],0)" "(p', q')" "wts_to_monoidLTS (intersff ts1 ts2)" "(w1', d2)" "(p2, q2)"]
+      using pq1_pq' pq'_pq2 monoid_rtrancl_into_rtrancl_rev[of "(p1, q1)" "([\<alpha>],0)" "(p', q')" "wts_to_monoidLTS (w_inters ts1 ts2)" "(w1', d2)" "(p2, q2)"]
       by simp
   next
     assume "(\<exists>p' d. (p1, ([\<alpha>], d), p') \<in> wts_to_monoidLTS ts1 \<and> (p', (w1',0), p2) \<in> monoid_rtrancl (wts_to_monoidLTS ts1))"
@@ -932,12 +933,12 @@ proof (induction w arbitrary: p1 q1 d)
       "(q1, ([\<alpha>], X), q') \<in> wts_to_monoidLTS ts2"
       "(q', (w1', Y), q2) \<in> monoid_rtrancl (wts_to_monoidLTS ts2)"
       using Cons(3) monoid_rtrancl_wts_to_monoidLTS_cases_rev by fastforce
-    obtain d1 where d1_p: "((p1,q1), ([\<alpha>], d1), (p',q')) \<in> wts_to_monoidLTS (intersff ts1 ts2)"
+    obtain d1 where d1_p: "((p1,q1), ([\<alpha>], d1), (p',q')) \<in> wts_to_monoidLTS (w_inters ts1 ts2)"
       using wts_to_monoidLTS_def by fastforce
-    have "((p',q'), (w1', 0), (p2,q2)) \<in> monoid_rtrancl (wts_to_monoidLTS (intersff ts1 ts2))"
+    have "((p',q'), (w1', 0), (p2,q2)) \<in> monoid_rtrancl (wts_to_monoidLTS (w_inters ts1 ts2))"
       using Cons(1)[of p' q'] p'_p(2) q'_p by blast
     then show ?thesis
-      using d1_p monoid_rtrancl_into_rtrancl_rev[of "(p1, q1)" "([\<alpha>],d1)" "(p', q')" "wts_to_monoidLTS (intersff ts1 ts2)" "(w1',0)" "(p2, q2)"]
+      using d1_p monoid_rtrancl_into_rtrancl_rev[of "(p1, q1)" "([\<alpha>],d1)" "(p', q')" "wts_to_monoidLTS (w_inters ts1 ts2)" "(w1',0)" "(p2, q2)"]
       by simp
   qed
 next
@@ -946,8 +947,8 @@ next
     by (metis fst_conv monoid_rtrancl.monoid_rtrancl_refl monoid_star_w0 mstar_wts_empty_one one_list_def one_prod_def)
 qed
 
-lemma intersff_sound_exi_fst:
-  assumes "((p1,q1), (w,d), (p2,q2)) \<in> monoid_rtrancl (wts_to_monoidLTS (intersff ts1 ts2))"
+lemma w_inters_sound_exi_fst:
+  assumes "((p1,q1), (w,d), (p2,q2)) \<in> monoid_rtrancl (wts_to_monoidLTS (w_inters ts1 ts2))"
   shows "\<exists>d'. (p1, (w,d'), p2) \<in> monoid_rtrancl (wts_to_monoidLTS ts1)"
   using assms 
 proof (induction rule: wts_to_monoidLTS_pair_induct)
@@ -963,10 +964,10 @@ next
     by auto
 qed
 
-lemma intersff_sound_non_zero_fst:
+lemma w_inters_sound_non_zero_fst:
   fixes ts1::"('state::finite, 'label::finite, 'weight::bounded_dioid) w_transitions"
   fixes ts2::"('state::finite, 'label, 'weight) w_transitions"
-  assumes "((p1,q1), (w,d), (p2,q2)) \<in> monoid_rtrancl (wts_to_monoidLTS (intersff ts1 ts2))"
+  assumes "((p1,q1), (w,d), (p2,q2)) \<in> monoid_rtrancl (wts_to_monoidLTS (w_inters ts1 ts2))"
   assumes "binary_aut ts1"
   assumes "d\<noteq>0"
   shows "(p1, (w,1), p2) \<in> monoid_rtrancl (wts_to_monoidLTS ts1)"
@@ -986,13 +987,13 @@ next
   then have "(p1, (w12, 1), p2) \<in> monoid_rtrancl (wts_to_monoidLTS ts1)"
     using d12_non0 step.IH step.prems(1) by blast
   moreover
-  have "(intersff ts1 ts2) $ ((p2, q2), hd w23, (p3, q3)) = d23"
+  have "(w_inters ts1 ts2) $ ((p2, q2), hd w23, (p3, q3)) = d23"
     using wts_label_d' step.hyps(2) by fastforce
   then obtain d23p d23q where
     "(p2, (w23, d23p), p3) \<in> (wts_to_monoidLTS ts1)"
     "(q2, (w23, d23q), q3) \<in> (wts_to_monoidLTS ts2)"
     "d23p * d23q = d23"
-    by (metis intersff_sound_transition step.hyps(2))
+    by (metis w_inters_sound_transition step.hyps(2))
   then have "(p2, (w23, 1), p3) \<in> wts_to_monoidLTS ts1"
     using binary_aut_transition_binary d23_non0 step.prems(1) by force
   ultimately
@@ -1001,8 +1002,8 @@ next
     by auto
 qed
 
-lemma intersff_sound_exi_snd:
-  assumes "((p1,q1), (w,d), (p2,q2)) \<in> monoid_rtrancl (wts_to_monoidLTS (intersff ts1 ts2))"
+lemma w_inters_sound_exi_snd:
+  assumes "((p1,q1), (w,d), (p2,q2)) \<in> monoid_rtrancl (wts_to_monoidLTS (w_inters ts1 ts2))"
   shows "\<exists>d'. (q1, (w,d'), q2) \<in> monoid_rtrancl (wts_to_monoidLTS ts2)"
   using assms
 proof (induction rule: wts_to_monoidLTS_pair_induct)
@@ -1018,10 +1019,10 @@ next
     by auto
 qed
 
-lemma intersff_sound_snd_non_zero:
+lemma w_inters_sound_snd_non_zero:
   fixes ts1::"('state::finite, 'label::finite, 'weight::bounded_dioid) w_transitions"
   fixes ts2::"('state::finite, 'label, 'weight) w_transitions"
-  assumes "((p1,q1), (w,d), (p2,q2)) \<in> monoid_rtrancl (wts_to_monoidLTS (intersff ts1 ts2))"
+  assumes "((p1,q1), (w,d), (p2,q2)) \<in> monoid_rtrancl (wts_to_monoidLTS (w_inters ts1 ts2))"
   assumes "binary_aut ts1"
   assumes "d\<noteq>0"
   shows "(q1, (w,d), q2) \<in> monoid_rtrancl (wts_to_monoidLTS ts2)"
@@ -1045,7 +1046,7 @@ next
     "(p2, (w23, d23p), p3) \<in> (wts_to_monoidLTS ts1)"
     "(q2, (w23, d23q), q3) \<in> (wts_to_monoidLTS ts2)"
     "d23p * d23q = d23"
-    by (metis intersff_sound_transition step.hyps(2))
+    by (metis w_inters_sound_transition step.hyps(2))
 
   have "d23p = 1"
     by (metis \<open>d23 \<noteq> 0\<close> d_mult_not_zero(1) f(1) f(3) binary_aut_transition_binary step.prems(1))
@@ -1057,10 +1058,10 @@ next
     by auto
 qed
 
-lemma intersff_sound_zero:
+lemma w_inters_sound_zero:
   fixes ts1::"('state::finite, 'label::finite, 'weight::bounded_dioid) w_transitions"
   fixes ts2::"('state::finite, 'label, 'weight) w_transitions"
-  assumes "((p1,q1), (w,d), (p2,q2)) \<in> monoid_rtrancl (wts_to_monoidLTS (intersff ts1 ts2))"
+  assumes "((p1,q1), (w,d), (p2,q2)) \<in> monoid_rtrancl (wts_to_monoidLTS (w_inters ts1 ts2))"
   assumes "binary_aut ts1"
   assumes "d=0"
   shows "(p1, (w,0), p2) \<in> monoid_rtrancl (wts_to_monoidLTS ts1) \<or>
@@ -1083,7 +1084,7 @@ next
       assume "(p1, (w12, 0),p2) \<in> monoid_rtrancl (wts_to_monoidLTS ts1)"
       moreover
       have "\<exists>dp23. (p2, (w23, dp23), p3) \<in> monoid_rtrancl (wts_to_monoidLTS ts1)"
-        by (meson intersff_sound_transition monoid_star_intros_step step.hyps(2))
+        by (meson w_inters_sound_transition monoid_star_intros_step step.hyps(2))
       ultimately
       have "(p1, ((w12 @ w23), 0), p3) \<in> monoid_rtrancl (wts_to_monoidLTS ts1)"
         using monoid_rtrancl_rtrancl_into_rtrancl[of p1 "(w12, 0)" p2 "(wts_to_monoidLTS ts1)" "(w23, _)" p3]
@@ -1094,7 +1095,7 @@ next
       assume "(q1, (w12, 0), q2) \<in> monoid_rtrancl (wts_to_monoidLTS ts2)"
       moreover
       have "\<exists>dq23. (q2, (w23, dq23), q3) \<in> monoid_rtrancl (wts_to_monoidLTS ts2)"
-        by (meson intersff_sound_transition monoid_star_intros_step step.hyps(2))
+        by (meson w_inters_sound_transition monoid_star_intros_step step.hyps(2))
       ultimately
       show ?thesis
         using monoid_rtrancl_rtrancl_into_rtrancl[of q1 "(w12, 0)" q2 "(wts_to_monoidLTS ts2)" "(w23, _)" q3]
@@ -1106,7 +1107,7 @@ next
     obtain d23p d23q where d23p_d23q_p: "(p2, (w23, d23p), p3) \<in> wts_to_monoidLTS ts1"
       "(q2, (w23, d23q), q3) \<in> wts_to_monoidLTS ts2"
       "d23 = d23p * d23q"
-      using intersff_sound_transition step.hyps(2) by blast
+      using w_inters_sound_transition step.hyps(2) by blast
     have d13zero: "d12 * d23 = 0"
       using snd_conv using step.prems(2) by blast
     have d23_split: "d23 = d23p * d23q"
@@ -1121,7 +1122,7 @@ next
         using True d23p_d23q_p(1) by blast
       moreover
       have "\<exists>dp12. (p1, (w12, dp12), p2) \<in> monoid_rtrancl (wts_to_monoidLTS ts1)"
-        using intersff_sound_non_zero_fst outer_outer_False step by blast
+        using w_inters_sound_non_zero_fst outer_outer_False step by blast
       ultimately
       have "(p1, (w12 @ w23, 0), p3) \<in> monoid_rtrancl (wts_to_monoidLTS ts1)"
         using monoid_rtrancl_into_rtrancl[of p1 "(w12,_)" p2 "(wts_to_monoidLTS ts1)"
@@ -1141,7 +1142,7 @@ next
           using True d23p_d23q_p(2) monoid_star_intros_step by blast
         moreover
         have "\<exists>dq12. (q1, (w12, dq12), q2) \<in> monoid_rtrancl (wts_to_monoidLTS ts2)"
-          using assms(2) outer_outer_False intersff_sound_snd_non_zero
+          using assms(2) outer_outer_False w_inters_sound_snd_non_zero
             step.hyps(1) by fastforce
         ultimately
         have "(q1, (w12 @ w23, 0), q3) \<in> monoid_rtrancl (wts_to_monoidLTS ts2)"
@@ -1155,7 +1156,7 @@ next
         have d23p_one: "d23p = 1"
           using d23p01 outer_False by auto
         have "(q1, (w12, d12), q2) \<in> monoid_rtrancl (wts_to_monoidLTS ts2)"
-          using intersff_sound_snd_non_zero outer_outer_False step.hyps(1)
+          using w_inters_sound_snd_non_zero outer_outer_False step.hyps(1)
             step.prems(1) by blast
         moreover
         have "(q2, (w23, d23q), q3) \<in> wts_to_monoidLTS ts2"
@@ -1170,27 +1171,27 @@ next
   qed
 qed
 
-lemma intersff_sound_and_complete:
+lemma w_inters_sound_and_complete:
   fixes ts1::"('state::finite, 'label::finite, 'weight::bounded_dioid) w_transitions"
   fixes ts2::"('state::finite, 'label, 'weight) w_transitions"
   assumes "binary_aut ts1"
-  shows "((p1,q1), (w,d), (p2,q2)) \<in> monoid_rtrancl (wts_to_monoidLTS (intersff ts1 ts2)) \<longleftrightarrow>
+  shows "((p1,q1), (w,d), (p2,q2)) \<in> monoid_rtrancl (wts_to_monoidLTS (w_inters ts1 ts2)) \<longleftrightarrow>
            (\<exists>dp dq. (p1, (w,dp), p2) \<in> monoid_rtrancl (wts_to_monoidLTS ts1) \<and>
                      (q1, (w,dq), q2) \<in> monoid_rtrancl (wts_to_monoidLTS ts2) \<and> dp * dq = d)"
 proof (cases "d = 0")
   case True
   show ?thesis
   proof 
-    assume inter: "((p1, q1), (w, d), p2, q2) \<in> monoid_rtrancl (wts_to_monoidLTS (intersff ts1 ts2))"
+    assume inter: "((p1, q1), (w, d), p2, q2) \<in> monoid_rtrancl (wts_to_monoidLTS (w_inters ts1 ts2))"
     then have dis0: "(p1, (w, 0), p2) \<in> monoid_rtrancl (wts_to_monoidLTS ts1) \<or> (q1, (w, 0), q2) \<in> monoid_rtrancl (wts_to_monoidLTS ts2)"
       using True
-      using intersff_sound_zero[of p1 q1 w d p2 q2 ts1 ts2] assms by auto
+      using w_inters_sound_zero[of p1 q1 w d p2 q2 ts1 ts2] assms by auto
     moreover
     have p1p2: "\<exists>dp. (p1, (w, dp), p2) \<in> monoid_rtrancl (wts_to_monoidLTS ts1)"
-      using intersff_sound_exi_fst[of p1 q1 w d p2, OF inter] by auto
+      using w_inters_sound_exi_fst[of p1 q1 w d p2, OF inter] by auto
     moreover
     have "\<exists>dq. (q1, (w, dq), q2) \<in> monoid_rtrancl (wts_to_monoidLTS ts2)"
-      by (meson inter intersff_sound_exi_snd)
+      by (meson inter w_inters_sound_exi_snd)
     ultimately
     show "\<exists>dp dq. (p1, (w, dp), p2) \<in> monoid_rtrancl (wts_to_monoidLTS ts1) \<and> (q1, (w, dq), q2) \<in> monoid_rtrancl (wts_to_monoidLTS ts2) \<and> dp * dq = d"
       using True mult_not_zero by blast
@@ -1201,16 +1202,16 @@ proof (cases "d = 0")
       "(q1, (w, dq), q2) \<in> monoid_rtrancl (wts_to_monoidLTS ts2)"
       "dp * dq = d"
       by auto
-    then show "((p1, q1), (w, d), p2, q2) \<in> monoid_rtrancl (wts_to_monoidLTS (intersff ts1 ts2))"
-      using assms binary_aut_path_binary intersff_complete_0 intersff_complete_1 by fastforce 
+    then show "((p1, q1), (w, d), p2, q2) \<in> monoid_rtrancl (wts_to_monoidLTS (w_inters ts1 ts2))"
+      using assms binary_aut_path_binary w_inters_complete_0 w_inters_complete_1 by fastforce 
   qed
 next
   case False
   show ?thesis
   proof 
-    assume "((p1, q1), (w, d), p2, q2) \<in> monoid_rtrancl (wts_to_monoidLTS (intersff ts1 ts2))"
+    assume "((p1, q1), (w, d), p2, q2) \<in> monoid_rtrancl (wts_to_monoidLTS (w_inters ts1 ts2))"
     show "\<exists>dp dq. (p1, (w, dp), p2) \<in> monoid_rtrancl (wts_to_monoidLTS ts1) \<and> (q1, (w, dq), q2) \<in> monoid_rtrancl (wts_to_monoidLTS ts2) \<and> dp * dq = d"
-      by (meson False \<open>((p1, q1), (w, d), p2, q2) \<in> monoid_rtrancl (wts_to_monoidLTS (intersff ts1 ts2))\<close> assms intersff_sound_non_zero_fst intersff_sound_snd_non_zero mult_1)
+      by (meson False \<open>((p1, q1), (w, d), p2, q2) \<in> monoid_rtrancl (wts_to_monoidLTS (w_inters ts1 ts2))\<close> assms w_inters_sound_non_zero_fst w_inters_sound_snd_non_zero mult_1)
   next 
     assume "\<exists>dp dq. (p1, (w, dp), p2) \<in> monoid_rtrancl (wts_to_monoidLTS ts1) \<and> (q1, (w, dq), q2) \<in> monoid_rtrancl (wts_to_monoidLTS ts2) \<and> dp * dq = d"
     then obtain dp dq where
@@ -1218,60 +1219,60 @@ next
       "(q1, (w, dq), q2) \<in> monoid_rtrancl (wts_to_monoidLTS ts2)"
       "dp * dq = d"
       by auto
-    then show "((p1, q1), (w, d), p2, q2) \<in> monoid_rtrancl (wts_to_monoidLTS (intersff ts1 ts2))"
-      using False assms binary_aut_path_binary intersff_complete_1 by fastforce
+    then show "((p1, q1), (w, d), p2, q2) \<in> monoid_rtrancl (wts_to_monoidLTS (w_inters ts1 ts2))"
+      using False assms binary_aut_path_binary w_inters_complete_1 by fastforce
   qed
 qed
 
-lemma intersff_sound:
+lemma w_inters_sound:
   fixes ts1::"('state::finite, 'label::finite, 'weight::bounded_dioid) w_transitions"
   fixes ts2::"('state::finite, 'label, 'weight) w_transitions"
   assumes "binary_aut ts1"
-  assumes "((p1,q1), (w,d), (p2,q2)) \<in> monoid_rtrancl (wts_to_monoidLTS (intersff ts1 ts2))"
+  assumes "((p1,q1), (w,d), (p2,q2)) \<in> monoid_rtrancl (wts_to_monoidLTS (w_inters ts1 ts2))"
   shows "(\<exists>dp dq. (p1, (w,dp), p2) \<in> monoid_rtrancl (wts_to_monoidLTS ts1) \<and>
                   (q1, (w,dq), q2) \<in> monoid_rtrancl (wts_to_monoidLTS ts2) \<and> dp * dq = d)"
-  using intersff_sound_and_complete assms by metis
+  using w_inters_sound_and_complete assms by metis
 
-lemma intersff_complete:
+lemma w_inters_complete:
   fixes ts1::"('state::finite, 'label::finite, 'weight::bounded_dioid) w_transitions"
   fixes ts2::"('state::finite, 'label, 'weight) w_transitions"
   assumes "binary_aut ts1"
   assumes "(p1, (w,dp), p2) \<in> monoid_rtrancl (wts_to_monoidLTS ts1)"
   assumes "(q1, (w,dq), q2) \<in> monoid_rtrancl (wts_to_monoidLTS ts2)"
-  shows "((p1,q1), (w,dp * dq), (p2,q2)) \<in> monoid_rtrancl (wts_to_monoidLTS (intersff ts1 ts2))"
-  using intersff_sound_and_complete assms by metis
+  shows "((p1,q1), (w,dp * dq), (p2,q2)) \<in> monoid_rtrancl (wts_to_monoidLTS (w_inters ts1 ts2))"
+  using w_inters_sound_and_complete assms by metis
 
-lemma intersff_sound_wts_to_weightLTS:
+lemma w_inters_sound_wts_to_weightLTS:
   fixes ts1::"('state::finite, 'label::finite, 'weight::bounded_dioid) w_transitions"
   fixes ts2::"('state::finite, 'label, 'weight) w_transitions"
   assumes "binary_aut ts1"
-  assumes "((p1,q1), d, (p2,q2)) \<in> monoid_rtrancl (wts_to_weightLTS (intersff ts1 ts2))"
+  assumes "((p1,q1), d, (p2,q2)) \<in> monoid_rtrancl (wts_to_weightLTS (w_inters ts1 ts2))"
   shows "(\<exists>dp dq. (p1, dp, p2) \<in> monoid_rtrancl (wts_to_weightLTS ts1) \<and>
          (q1, dq, q2) \<in> monoid_rtrancl (wts_to_weightLTS ts2) \<and> dp * dq = d)"  
-  using assms wts_weightLTS_star_to_monoidLTS_star[of "(p1,q1)" d "(p2,q2)" "intersff ts1 ts2"]
-        intersff_sound[OF assms(1), of p1 q1 _ d p2 q2 ts2] wts_monoidLTS_star_to_weightLTS_star
+  using assms wts_weightLTS_star_to_monoidLTS_star[of "(p1,q1)" d "(p2,q2)" "w_inters ts1 ts2"]
+        w_inters_sound[OF assms(1), of p1 q1 _ d p2 q2 ts2] wts_monoidLTS_star_to_weightLTS_star
   by meson
 
-lemma intersff_sound_wts_to_monoidLTS:
+lemma w_inters_sound_wts_to_monoidLTS:
   fixes ts1::"('state::finite, 'label::finite, 'weight::bounded_dioid) w_transitions"
   fixes ts2::"('state::finite, 'label, 'weight) w_transitions"
   assumes "binary_aut ts1"
-  assumes "((p1,q1), d, (p2,q2)) \<in> monoid_rtrancl (wts_to_weightLTS (intersff ts1 ts2))"
+  assumes "((p1,q1), d, (p2,q2)) \<in> monoid_rtrancl (wts_to_weightLTS (w_inters ts1 ts2))"
   shows "(\<exists>w dp dq. (p1, (w,dp), p2) \<in> monoid_rtrancl (wts_to_monoidLTS ts1) \<and>
                     (q1, (w,dq), q2) \<in> monoid_rtrancl (wts_to_monoidLTS ts2) \<and> dp * dq = d)"
-  using wts_weightLTS_star_to_monoidLTS_star[of "(p1,q1)" d "(p2,q2)" "intersff ts1 ts2"]
-        intersff_sound[OF assms(1), of p1 q1 _ d p2 q2 ts2] assms(2)
+  using wts_weightLTS_star_to_monoidLTS_star[of "(p1,q1)" d "(p2,q2)" "w_inters ts1 ts2"]
+        w_inters_sound[OF assms(1), of p1 q1 _ d p2 q2 ts2] assms(2)
   by meson
 
-lemma intersff_complete_wts_to_weightLTS:
+lemma w_inters_complete_wts_to_weightLTS:
   fixes ts1::"('state::finite, 'label::finite, 'weight::bounded_dioid) w_transitions"
   fixes ts2::"('state::finite, 'label, 'weight) w_transitions"
   assumes "binary_aut ts1"
   assumes "(p1, (w, dp), p2) \<in> monoid_rtrancl (wts_to_monoidLTS ts1)"
   assumes "(q1, (w, dq), q2) \<in> monoid_rtrancl (wts_to_monoidLTS ts2)"
-  shows "((p1, q1), dp * dq, (p2, q2)) \<in> monoid_rtrancl (wts_to_weightLTS (intersff ts1 ts2))"
-  using intersff_complete[OF assms(1)] assms(2,3)
-        wts_monoidLTS_star_to_weightLTS_star[of "(p1,q1)" w "dp * dq" "(p2,q2)" "intersff ts1 ts2"]
+  shows "((p1, q1), dp * dq, (p2, q2)) \<in> monoid_rtrancl (wts_to_weightLTS (w_inters ts1 ts2))"
+  using w_inters_complete[OF assms(1)] assms(2,3)
+        wts_monoidLTS_star_to_weightLTS_star[of "(p1,q1)" w "dp * dq" "(p2,q2)" "w_inters ts1 ts2"]
   by fast
 
 definition "fst_trans_all = fin_fun_of_fun fst_trans"
